src/ExtractionHaskell/word_by_word_montgomery_generic.v
@@ -1,0 +1,4 @@
+Require Import Crypto.StandaloneHaskellMain.
+
+(*Redirect "/tmp/word_by_word_montgomery.hs" *)Recursive Extraction WordByWordMontgomery.main.
+(* cat /tmp/word_by_word_montgomery.hs.out | sed -f haskell.sed  > ../../word_by_word_montgomery.hs *)
