src/ExtractionOCaml/word_by_word_montgomery_generic.v
@@ -1,0 +1,3 @@
+Require Import Crypto.StandaloneOCamlMain.
+
+(*Redirect "/tmp/word_by_word_montgomery.ml"*) Recursive Extraction WordByWordMontgomery.main.
