src/PushButtonSynthesis/WordByWordMontgomeryGeneric.v
@@ -1,0 +1,1119 @@
+(** * Push-Button Synthesis of Word-By-Word Montgomery *)
+Require Import Coq.Strings.String.
+Require Import Coq.micromega.Lia.
+Require Import Coq.ZArith.ZArith.
+Require Import Coq.MSets.MSetPositive.
+Require Import Coq.Lists.List.
+Require Import Coq.QArith.QArith_base Coq.QArith.Qround.
+Require Import Coq.Program.Tactics. (* For WBW Montgomery proofs *)
+Require Import Coq.derive.Derive.
+Require Import Crypto.Util.ErrorT.
+Require Import Crypto.Util.ListUtil.
+Require Import Crypto.Util.ListUtil.FoldBool.
+Require Import Crypto.Util.Strings.Decimal.
+Require Import Crypto.Util.ZRange.
+Require Import Crypto.Util.ZUtil.Definitions.
+Require Import Crypto.Util.ZUtil.Zselect.
+Require Import Crypto.Util.ZUtil.Tactics.LtbToLt.
+Require Import Crypto.Util.ZUtil.ModInv. (* Only needed for WBW Montgomery *)
+Require Import Crypto.Util.ZUtil.Modulo. (* Only needed for WBW Montgomery proofs *)
+Require Import Crypto.Util.ZUtil.Le. (* Only needed for WBW Montgomery proofs *)
+Require Import Crypto.Util.Prod. (* For WBW Montgomery proofs *)
+Require Import Crypto.Util.ZUtil.Tactics.PullPush.Modulo. (* For WBW montgomery proofs *)
+Require Import Crypto.Util.ZUtil.Tactics.RewriteModSmall. (* For WBW montgomery proofs *)
+Require Import Crypto.Util.ZUtil.Div. (* For WBW Montgomery proofs *)
+Require Import Crypto.Util.ZUtil.Tactics.DivModToQuotRem. (* For WBW Montgomery proofs *)
+Require Import Crypto.Util.ZUtil.Ones. (* For WBW montgomery proofs *)
+Require Import Crypto.Util.ZUtil.Shift. (* For WBW montgomery proofs *)
+Require Import Crypto.Util.ZUtil.ModExp.
+Require Import Crypto.Util.Tactics.HasBody.
+Require Import Crypto.Util.Tactics.Head.
+Require Import Crypto.Util.Tactics.SpecializeBy.
+Require Import Rewriter.Language.Wf.
+Require Import Crypto.Language.WfExtra.
+Require Import Rewriter.Language.Language.
+Require Import Crypto.Language.API.
+Require Import Crypto.AbstractInterpretation.AbstractInterpretation.
+Require Import Crypto.Stringification.Language.
+Require Import Crypto.Arithmetic.Core.
+Require Import Crypto.Arithmetic.ModOps.
+Require Import Crypto.Arithmetic.Freeze.
+Require Import Crypto.Arithmetic.Partition.
+Require Import Crypto.Arithmetic.WordByWordMontgomery.
+Require Import Crypto.Arithmetic.UniformWeight.
+Require Import Crypto.Arithmetic.BYInv.
+Require Import Crypto.BoundsPipeline.
+Require Import Crypto.COperationSpecifications.
+Require Import Crypto.PushButtonSynthesis.ReificationCache.
+Require Import Crypto.PushButtonSynthesis.Primitives.
+Require Import Crypto.PushButtonSynthesis.WordByWordMontgomeryReificationCache.
+Require Import Crypto.PushButtonSynthesis.BYInversionReificationCache.
+Require Import Crypto.Assembly.Equivalence.
+Import ListNotations.
+Local Open Scope Z_scope. Local Open Scope list_scope. Local Open Scope bool_scope.
+
+Import
+  Language.Wf.Compilers
+  Language.WfExtra.Compilers
+  Language.Compilers
+  AbstractInterpretation.Compilers
+  Stringification.Language.Compilers.
+Import Compilers.API.
+
+Import COperationSpecifications.Primitives.
+Import COperationSpecifications.Solinas.
+Import COperationSpecifications.WordByWordMontgomery.
+
+Import Associational Positional.
+Import Arithmetic.WordByWordMontgomery.WordByWordMontgomery.
+
+Import WordByWordMontgomeryReificationCache.WordByWordMontgomery.
+Import BYInversionReificationCache.WordByWordMontgomeryInversion.
+
+Local Coercion Z.of_nat : nat >-> Z.
+Local Coercion QArith_base.inject_Z : Z >-> Q.
+Local Coercion Z.pos : positive >-> Z.
+
+Local Set Keyed Unification. (* needed for making [autorewrite] fast, c.f. COQBUG(https://github.com/coq/coq/issues/9283) *)
+
+(* needed for making [autorewrite] not take a very long time *)
+Local Opaque
+      reified_mul_gen
+      reified_add_gen
+      reified_sub_gen
+      reified_opp_gen
+      reified_to_bytes_gen
+      reified_from_bytes_gen
+      reified_nonzero_gen
+      reified_square_gen
+      reified_encode_gen
+      reified_from_montgomery_gen
+      reified_to_montgomery_gen
+      reified_zero_gen
+      reified_one_gen
+      expr.Interp.
+
+Section __.
+  Context {output_language_api : ToString.OutputLanguageAPI}
+          {language_naming_conventions : language_naming_conventions_opt}
+          {documentation_options : documentation_options_opt}
+          {package_namev : package_name_opt}
+          {class_namev : class_name_opt}
+          {static : static_opt}
+          {internal_static : internal_static_opt}
+          {low_level_rewriter_method : low_level_rewriter_method_opt}
+          {only_signed : only_signed_opt}
+          {no_select : no_select_opt}
+          {use_mul_for_cmovznz : use_mul_for_cmovznz_opt}
+          {emit_primitives : emit_primitives_opt}
+          {should_split_mul : should_split_mul_opt}
+          {should_split_multiret : should_split_multiret_opt}
+          {unfold_value_barrier : unfold_value_barrier_opt}
+          {assembly_hints_lines : assembly_hints_lines_opt}
+          {widen_carry : widen_carry_opt}
+          {widen_bytes : widen_bytes_opt}
+          {assembly_calling_registers : assembly_calling_registers_opt}
+          {assembly_stack_size : assembly_stack_size_opt}
+          {error_on_unused_assembly_functions : error_on_unused_assembly_functions_opt}
+          {assembly_output_first : assembly_output_first_opt}
+          {assembly_argument_registers_left_to_right : assembly_argument_registers_left_to_right_opt}
+          (m : Z)
+          (machine_wordsize : Z).
+
+  Definition s := 2^Z.log2_up m.
+  Definition c := s - m.
+  Definition n : nat := Z.to_nat (Qceiling (Z.log2_up s / machine_wordsize)).
+  Definition sat_limbs := (n + 1)%nat.   (* to represent m in twos complement we might need another bit *)
+  Definition r := 2^machine_wordsize.
+  Definition r'
+    := match Z.modinv r m with
+       | Some r' => r'
+       | None => 0
+       end.
+  Definition m'
+    := match Z.modinv (-m) r with
+       | Some m' => m'
+       | None => 0
+       end.
+  Definition n_bytes := bytes_n s.
+
+  Definition divstep_precompmod :=
+    let bits := (Z.log2 m) + 1 in
+    let i := if bits <? 46 then (49 * bits + 80) / 17 else (49 * bits + 57) / 17 in
+    let k := (m + 1) / 2 in
+    (Z.modexp k i m).
+
+  Definition prime_upperbound_list : list Z
+    := Partition.partition (uweight machine_wordsize) n (s-1).
+  Definition prime_bytes_upperbound_list : list Z
+    := Partition.partition (weight 8 1) n_bytes (s-1).
+  Definition upperbounds : list Z := prime_upperbound_list.
+  Definition prime_bound : ZRange.type.interp (base.type.Z)
+    := r[0~>m-1]%zrange.
+  Definition prime_bounds : list (ZRange.type.option.interp base.type.Z)
+    := List.map (fun v => Some r[0 ~> v]%zrange) prime_upperbound_list.
+  Definition prime_bytes_bounds : list (ZRange.type.option.interp (base.type.Z))
+    := List.map (fun v => Some r[0 ~> v]%zrange) prime_bytes_upperbound_list.
+  Local Notation saturated_bounds := (saturated_bounds n machine_wordsize).
+  Local Notation larger_saturated_bounds := (Primitives.saturated_bounds sat_limbs machine_wordsize).
+
+  Definition divstep_input :=
+    (Some r[0~>2^machine_wordsize-1],
+     (Some (repeat (Some r[0 ~> 2^machine_wordsize-1]) sat_limbs),
+      (Some (repeat (Some r[0 ~> 2^machine_wordsize-1]) sat_limbs),
+       (Some (repeat (Some r[0 ~> 2^machine_wordsize-1]) n),
+        (Some (repeat (Some r[0 ~> 2^machine_wordsize-1]) n),tt)))))%zrange.
+
+  Definition divstep_output :=
+    (Some r[0~>2^machine_wordsize-1],
+     Some (repeat (Some r[0 ~> 2^machine_wordsize-1]) sat_limbs),
+     Some (repeat (Some r[0 ~> 2^machine_wordsize-1]) sat_limbs),
+     Some (repeat (Some r[0 ~> 2^machine_wordsize-1]) n),
+     Some (repeat (Some r[0 ~> 2^machine_wordsize-1]) n))%zrange.
+
+  (* We include [0], so that even after bounds relaxation, we can
+       notice where the constant 0s are, and remove them. *)
+  Definition possible_values_of_machine_wordsize
+    := prefix_with_carry [machine_wordsize; 2 * machine_wordsize]%Z.
+
+  Definition possible_values_of_machine_wordsize_with_bytes
+    := prefix_with_carry_bytes [machine_wordsize; 2 * machine_wordsize]%Z.
+
+  Let possible_values := possible_values_of_machine_wordsize.
+  Let possible_values_with_bytes := possible_values_of_machine_wordsize_with_bytes.
+  Definition bounds : list (ZRange.type.option.interp base.type.Z)
+    := saturated_bounds (*List.map (fun u => Some r[0~>u]%zrange) upperbounds*).
+  Definition larger_bounds : list (ZRange.type.option.interp base.type.Z)
+    := larger_saturated_bounds (*List.map (fun u => Some r[0~>u]%zrange) upperbounds*).
+
+  Local Instance no_select_size : no_select_size_opt := no_select_size_of_no_select machine_wordsize.
+  Local Instance split_mul_to : split_mul_to_opt := split_mul_to_of_should_split_mul machine_wordsize possible_values.
+  Local Instance split_multiret_to : split_multiret_to_opt := split_multiret_to_of_should_split_multiret machine_wordsize possible_values.
+
+  (** Note: If you change the name or type signature of this
+        function, you will need to update the code in CLI.v *)
+  Definition check_args {T} (requests : list string) (res : Pipeline.ErrorT T)
+    : Pipeline.ErrorT T
+    := check_args_of_list
+         (List.map
+            (fun v => (true, v))
+            [((1 <? machine_wordsize)%Z, Pipeline.Value_not_ltZ "machine_wordsize <= 1" 1 machine_wordsize)
+             ; ((0 <? c)%Z, Pipeline.Value_not_ltZ "c ≤ 0" 0 c)
+             ; ((1 <? m)%Z, Pipeline.Value_not_ltZ "m ≤ 1" 1 m)
+             ; (negb (n =? 0)%nat, Pipeline.Values_not_provably_distinctZ "n = 0" n 0%nat)
+             ; (negb (r' =? 0)%Z, Pipeline.No_modular_inverse "r⁻¹ mod m" r m)
+             ; (((r * r') mod m =? 1)%Z, Pipeline.Values_not_provably_equalZ "(r * r') mod m ≠ 1" ((r * r') mod m) 1)
+             ; (((m * m') mod r =? (-1) mod r)%Z, Pipeline.Values_not_provably_equalZ "(m * m') mod r ≠ (-1) mod r" ((m * m') mod r) ((-1) mod r))
+             ; (s <=? r^n, Pipeline.Value_not_leZ "r^n ≤ s" s (r^n))
+             ; (s <=? uweight machine_wordsize n, Pipeline.Value_not_leZ "weight n < s (needed for from_bytes)" s (uweight machine_wordsize n))
+             ; (s <=? uweight 8 n_bytes, Pipeline.Value_not_leZ "bytes_weight n_bytes < s (needed for from_bytes)" s (uweight 8 n_bytes))
+         ])
+         res.
+
+  Local Arguments Z.mul !_ !_.
+
+  Local Ltac use_curve_good_t :=
+    repeat first [ use_requests_to_prove_curve_good_t_step
+                 | assumption
+                 | lia
+                 | progress autorewrite with distr_length
+                 | progress distr_length
+                 | solve [ auto with zarith ]
+                 | rewrite Z.log2_pow2 by use_curve_good_t ].
+
+  Context (requests : list string)
+          (curve_good : check_args requests (Success tt) = Success tt).
+
+  Lemma use_curve_good
+    : Z.pos (Z.to_pos m) = m
+      /\ m = s - c
+      /\ Z.pos (Z.to_pos m) <> 0
+      /\ s - c <> 0
+      /\ 0 < s
+      /\ s <> 0
+      /\ 0 < machine_wordsize
+      /\ n <> 0%nat
+      /\ List.length bounds = n
+      /\ 0 < 1 <= machine_wordsize
+      /\ 0 < c < s
+      /\ (r * r') mod m = 1
+      /\ (m * m') mod r = (-1) mod r
+      /\ 0 < machine_wordsize
+      /\ 1 < m
+      /\ m < r^n
+      /\ s = 2^Z.log2 s
+      /\ s <= uweight machine_wordsize n
+      /\ s <= uweight 8 n_bytes.
+  Proof.
+    prepare_use_curve_good (); cbv [s c] in *.
+    { destruct m eqn:?; cbn; lia. }
+    { use_curve_good_t. }
+    { use_curve_good_t. }
+    { use_curve_good_t. }
+    { use_curve_good_t. }
+    { use_curve_good_t. }
+    { use_curve_good_t. }
+    { use_curve_good_t. }
+    { use_curve_good_t. }
+    { use_curve_good_t. }
+    { use_curve_good_t. }
+    { use_curve_good_t. }
+    { use_curve_good_t. }
+  Qed.
+
+  Local Notation valid := (valid machine_wordsize n m).
+  Local Notation bytes_valid := (WordByWordMontgomery.valid 8 n_bytes m).
+
+  Local Notation from_montgomery_res := (from_montgomerymod machine_wordsize n m m').
+
+  Local Notation notations_for_docstring prefix
+    := ((CorrectnessStringification.dyn_context.cons
+           m "m"
+           (CorrectnessStringification.dyn_context.cons
+              r' ("((2^" ++ Decimal.Z.to_string machine_wordsize ++ ")⁻¹ mod m)")
+              (CorrectnessStringification.dyn_context.cons
+                 from_montgomery_res "from_montgomery"
+                 (CorrectnessStringification.dyn_context.cons
+                    (@eval machine_wordsize n) "eval"
+                    (CorrectnessStringification.dyn_context.cons
+                       (@eval 8 n_bytes) "bytes_eval"
+                            (CorrectnessStringification.dyn_context.cons
+                               (Z.log2 m) "(log2 m)"
+                               (CorrectnessStringification.dyn_context.cons
+                                  (@eval_twos_complement machine_wordsize n) "twos_complement_eval"
+                                  CorrectnessStringification.dyn_context.nil)))))))%string)
+         (only parsing).
+  Local Notation "'docstring_with_summary_from_lemma!' prefix summary correctness"
+    := (docstring_with_summary_from_lemma_with_ctx!
+          (notations_for_docstring prefix)
+          summary
+          correctness)
+         (only parsing, at level 10, prefix at next level, summary at next level, correctness at next level).
+
+  Definition mul
+    := Pipeline.BoundsPipeline
+         false (* subst01 *)
+         None (* fancy *)
+         possible_values
+         (reified_mul_gen
+            @ GallinaReify.Reify machine_wordsize @ GallinaReify.Reify n @ GallinaReify.Reify m @ GallinaReify.Reify m')
+         (Some bounds, (Some bounds, tt))
+         (Some bounds).
+
+  Definition smul (prefix : string)
+    : string * (Pipeline.ErrorT (Pipeline.ExtendedSynthesisResult _))
+    := Eval cbv beta in
+        FromPipelineToString
+          machine_wordsize prefix "mul" mul
+          (docstring_with_summary_from_lemma!
+             prefix
+             (fun fname : string => [text_before_function_name ++ fname ++ " multiplies two field elements in the Montgomery domain."]%string)
+             (mul_correct machine_wordsize n m valid from_montgomery_res)).
+
+  Definition square
+    := Pipeline.BoundsPipeline
+         false (* subst01 *)
+         None (* fancy *)
+         possible_values
+         (reified_square_gen
+            @ GallinaReify.Reify machine_wordsize @ GallinaReify.Reify n @ GallinaReify.Reify m @ GallinaReify.Reify m')
+         (Some bounds, tt)
+         (Some bounds).
+
+  Definition ssquare (prefix : string)
+    : string * (Pipeline.ErrorT (Pipeline.ExtendedSynthesisResult _))
+    := Eval cbv beta in
+        FromPipelineToString
+          machine_wordsize prefix "square" square
+          (docstring_with_summary_from_lemma!
+             prefix
+             (fun fname : string => [text_before_function_name ++ fname ++ " squares a field element in the Montgomery domain."]%string)
+             (square_correct machine_wordsize n m valid from_montgomery_res)).
+
+  Definition add
+    := Pipeline.BoundsPipeline
+         true (* subst01 *)
+         None (* fancy *)
+         possible_values
+         (reified_add_gen
+            @ GallinaReify.Reify machine_wordsize @ GallinaReify.Reify n @ GallinaReify.Reify m)
+         (Some bounds, (Some bounds, tt))
+         (Some bounds).
+
+  Definition sadd (prefix : string)
+    : string * (Pipeline.ErrorT (Pipeline.ExtendedSynthesisResult _))
+    := Eval cbv beta in
+        FromPipelineToString
+          machine_wordsize prefix "add" add
+          (docstring_with_summary_from_lemma!
+             prefix
+             (fun fname : string => [text_before_function_name ++ fname ++ " adds two field elements in the Montgomery domain."]%string)
+             (add_correct machine_wordsize n m valid from_montgomery_res)).
+
+  Definition sub
+    := Pipeline.BoundsPipeline
+         true (* subst01 *)
+         None (* fancy *)
+         possible_values
+         (reified_sub_gen
+            @ GallinaReify.Reify machine_wordsize @ GallinaReify.Reify n @ GallinaReify.Reify m)
+         (Some bounds, (Some bounds, tt))
+         (Some bounds).
+
+  Definition ssub (prefix : string)
+    : string * (Pipeline.ErrorT (Pipeline.ExtendedSynthesisResult _))
+    := Eval cbv beta in
+        FromPipelineToString
+          machine_wordsize prefix "sub" sub
+          (docstring_with_summary_from_lemma!
+             prefix
+             (fun fname : string => [text_before_function_name ++ fname ++ " subtracts two field elements in the Montgomery domain."]%string)
+             (sub_correct machine_wordsize n m valid from_montgomery_res)).
+
+  Definition opp
+    := Pipeline.BoundsPipeline
+         true (* subst01 *)
+         None (* fancy *)
+         possible_values
+         (reified_opp_gen
+            @ GallinaReify.Reify machine_wordsize @ GallinaReify.Reify n @ GallinaReify.Reify m)
+         (Some bounds, tt)
+         (Some bounds).
+
+  Definition sopp (prefix : string)
+    : string * (Pipeline.ErrorT (Pipeline.ExtendedSynthesisResult _))
+    := Eval cbv beta in
+        FromPipelineToString
+          machine_wordsize prefix "opp" opp
+          (docstring_with_summary_from_lemma!
+             prefix
+             (fun fname : string => [text_before_function_name ++ fname ++ " negates a field element in the Montgomery domain."]%string)
+             (opp_correct machine_wordsize n m valid from_montgomery_res)).
+
+  Definition from_montgomery
+    := Pipeline.BoundsPipeline
+         true (* subst01 *)
+         None (* fancy *)
+         possible_values
+         (reified_from_montgomery_gen
+            @ GallinaReify.Reify machine_wordsize @ GallinaReify.Reify n @ GallinaReify.Reify m @ GallinaReify.Reify m')
+         (Some bounds, tt)
+         (Some bounds).
+
+  Definition sfrom_montgomery (prefix : string)
+    : string * (Pipeline.ErrorT (Pipeline.ExtendedSynthesisResult _))
+    := Eval cbv beta in
+        FromPipelineToString
+          machine_wordsize prefix "from_montgomery" from_montgomery
+          (docstring_with_summary_from_lemma!
+             prefix
+             (fun fname : string => [text_before_function_name ++ fname ++ " translates a field element out of the Montgomery domain."]%string)
+             (from_montgomery_correct machine_wordsize n m r' valid)).
+
+  Definition to_montgomery
+    := Pipeline.BoundsPipeline
+         true (* subst01 *)
+         None (* fancy *)
+         possible_values
+         (reified_to_montgomery_gen
+            @ GallinaReify.Reify machine_wordsize @ GallinaReify.Reify n @ GallinaReify.Reify m @ GallinaReify.Reify m')
+         (Some bounds, tt)
+         (Some bounds).
+
+  Definition sto_montgomery (prefix : string)
+    : string * (Pipeline.ErrorT (Pipeline.ExtendedSynthesisResult _))
+    := Eval cbv beta in
+        FromPipelineToString
+          machine_wordsize prefix "to_montgomery" to_montgomery
+          (docstring_with_summary_from_lemma!
+             prefix
+             (fun fname : string => [text_before_function_name ++ fname ++ " translates a field element into the Montgomery domain."]%string)
+             (to_montgomery_correct machine_wordsize n m valid from_montgomery_res)).
+
+  Definition nonzero
+    := Pipeline.BoundsPipeline
+         true (* subst01 *)
+         None (* fancy *)
+         possible_values
+         reified_nonzero_gen
+         (Some bounds, tt)
+         (Some r[0~>r-1]%zrange).
+
+  Definition snonzero (prefix : string)
+    : string * (Pipeline.ErrorT (Pipeline.ExtendedSynthesisResult _))
+    := Eval cbv beta in
+        FromPipelineToString
+          machine_wordsize prefix "nonzero" nonzero
+          (docstring_with_summary_from_lemma!
+             prefix
+             (fun fname : string => [text_before_function_name ++ fname ++ " outputs a single non-zero word if the input is non-zero and zero otherwise."]%string)
+             (nonzero_correct machine_wordsize n m valid from_montgomery_res)).
+
+  Definition to_bytes
+    := Pipeline.BoundsPipeline
+         false (* subst01 *)
+         None (* fancy *)
+         possible_values_with_bytes
+         (reified_to_bytes_gen
+            @ GallinaReify.Reify machine_wordsize @ GallinaReify.Reify n @ GallinaReify.Reify m)
+         (Some prime_bounds, tt)
+         (Some prime_bytes_bounds).
+
+  Definition sto_bytes (prefix : string)
+    : string * (Pipeline.ErrorT (Pipeline.ExtendedSynthesisResult _))
+    := Eval cbv beta in
+        FromPipelineToString
+          machine_wordsize prefix "to_bytes" to_bytes
+          (docstring_with_summary_from_lemma!
+             prefix
+             (fun fname : string => [text_before_function_name ++ fname ++ " serializes a field element NOT in the Montgomery domain to bytes in little-endian order."]%string)
+             (to_bytes_correct machine_wordsize n n_bytes m valid)).
+
+  Definition from_bytes
+    := Pipeline.BoundsPipeline
+         false (* subst01 *)
+         None (* fancy *)
+         possible_values_with_bytes
+         (reified_from_bytes_gen
+            @ GallinaReify.Reify machine_wordsize @ GallinaReify.Reify 1 @ GallinaReify.Reify s @ GallinaReify.Reify n)
+         (Some prime_bytes_bounds, tt)
+         (Some prime_bounds).
+
+  Definition sfrom_bytes (prefix : string)
+    : string * (Pipeline.ErrorT (Pipeline.ExtendedSynthesisResult _))
+    := Eval cbv beta in
+        FromPipelineToString
+          machine_wordsize prefix "from_bytes" from_bytes
+          (docstring_with_summary_from_lemma!
+             prefix
+             (fun fname : string => [text_before_function_name ++ fname ++ " deserializes a field element NOT in the Montgomery domain from bytes in little-endian order."]%string)
+             (from_bytes_correct machine_wordsize n n_bytes m valid bytes_valid)).
+
+  Definition encode
+    := Pipeline.BoundsPipeline
+         true (* subst01 *)
+         None (* fancy *)
+         possible_values
+         (reified_encode_gen
+            @ GallinaReify.Reify machine_wordsize @ GallinaReify.Reify n @ GallinaReify.Reify m @ GallinaReify.Reify m')
+         (Some prime_bound, tt)
+         (Some bounds).
+
+  Definition sencode (prefix : string)
+    : string * (Pipeline.ErrorT (Pipeline.ExtendedSynthesisResult _))
+    := Eval cbv beta in
+        FromPipelineToString
+          machine_wordsize prefix "encode" encode
+          (docstring_with_summary_from_lemma!
+             prefix
+             (fun fname : string => [text_before_function_name ++ fname ++ " encodes an integer as a field element in the Montgomery domain."]%string)
+             (encode_correct machine_wordsize n m valid from_montgomery_res)).
+
+  Definition zero
+    := Pipeline.BoundsPipeline
+         true (* subst01 *)
+         None (* fancy *)
+         possible_values
+         (reified_zero_gen
+            @ GallinaReify.Reify machine_wordsize @ GallinaReify.Reify n @ GallinaReify.Reify m @ GallinaReify.Reify m')
+         tt
+         (Some bounds).
+
+  Definition szero (prefix : string)
+    : string * (Pipeline.ErrorT (Pipeline.ExtendedSynthesisResult _))
+    := Eval cbv beta in
+        FromPipelineToString
+          machine_wordsize prefix "zero" zero
+          (docstring_with_summary_from_lemma!
+             prefix
+             (fun fname => [text_before_function_name ++ fname ++ " returns the field element zero in the Montgomery domain."]%string)
+             (zero_correct machine_wordsize n m valid from_montgomery_res)).
+
+  Definition one
+    := Pipeline.BoundsPipeline
+         true (* subst01 *)
+         None (* fancy *)
+         possible_values
+         (reified_one_gen
+            @ GallinaReify.Reify machine_wordsize @ GallinaReify.Reify n @ GallinaReify.Reify m @ GallinaReify.Reify m')
+         tt
+         (Some bounds).
+
+  Definition sone (prefix : string)
+    : string * (Pipeline.ErrorT (Pipeline.ExtendedSynthesisResult _))
+    := Eval cbv beta in
+        FromPipelineToString
+          machine_wordsize prefix "set_one" one (* to avoid conflict with boringSSL *)
+          (docstring_with_summary_from_lemma!
+             prefix
+             (fun fname => [text_before_function_name ++ fname ++ " returns the field element one in the Montgomery domain."]%string)
+             (one_correct machine_wordsize n m valid from_montgomery_res)).
+
+  Definition reval (* r for reified *)
+    := Pipeline.RepeatRewriteAddAssocLeftAndFlattenThunkedRects
+         n
+         (Pipeline.PreBoundsPipeline
+            true (* subst01 *)
+            false (* let_bind_return *)
+            None (* fancy *)
+            (reified_eval_gen
+               @ GallinaReify.Reify machine_wordsize @ GallinaReify.Reify n)
+            (Some bounds, tt)).
+
+  Definition seval (arg_name : string) (* s for string *)
+    := Show.show (invert_expr.smart_App_curried (reval _) (arg_name, tt)).
+
+  Definition rbytes_eval (* r for reified *)
+    := Pipeline.RepeatRewriteAddAssocLeftAndFlattenThunkedRects
+         n_bytes
+         (Pipeline.PreBoundsPipeline
+            true (* subst01 *)
+            false (* let_bind_return *)
+            None (* fancy *)
+            (reified_bytes_eval_gen
+               @ GallinaReify.Reify s)
+            (Some prime_bytes_bounds, tt)).
+
+  Definition sbytes_eval (arg_name : string) (* s for string *)
+    := Show.show (invert_expr.smart_App_curried (rbytes_eval _) (arg_name, tt)).
+
+  Definition reval_twos_complement (* r for reified *)
+    := Pipeline.RepeatRewriteAddAssocLeftAndFlattenThunkedRects
+         n
+         (Pipeline.PreBoundsPipeline
+            true (* subst01 *)
+            false (* let_bind_return *)
+            None (* fancy *)
+            (reified_eval_twos_complement_gen
+               @ GallinaReify.Reify machine_wordsize
+               @ GallinaReify.Reify n)
+            (Some bounds, tt)).
+
+  Definition seval_twos_complement (arg_name : string) (* s for string *)
+    := Show.show (invert_expr.smart_App_curried (reval_twos_complement _) (arg_name, tt)).
+
+  Definition selectznz : Pipeline.ErrorT _ := Primitives.selectznz n machine_wordsize.
+  Definition sselectznz (prefix : string)
+    : string * (Pipeline.ErrorT (Pipeline.ExtendedSynthesisResult _))
+    := Primitives.sselectznz n machine_wordsize prefix.
+
+  Definition msat
+    := Pipeline.BoundsPipeline
+         true (* subst01 *)
+         None (* fancy *)
+         possible_values
+         (reified_msat_gen
+            @ GallinaReify.Reify machine_wordsize @ GallinaReify.Reify sat_limbs @ GallinaReify.Reify m)
+         tt
+         (Some larger_bounds).
+
+ Definition smsat (prefix : string)
+    : string * (Pipeline.ErrorT (Pipeline.ExtendedSynthesisResult _))
+    := Eval cbv beta in
+        FromPipelineToString
+          machine_wordsize prefix "msat" msat
+          (docstring_with_summary_from_lemma!
+             prefix
+             (fun fname => [text_before_function_name ++ fname ++ " returns the saturated representation of the prime modulus."]%string)
+             (msat_correct machine_wordsize n m valid)).
+
+  Definition divstep_precomp
+    := Pipeline.BoundsPipeline
+         true (* subst01 *)
+         None (* fancy *)
+         possible_values
+         (reified_encode_gen
+            @ GallinaReify.Reify machine_wordsize @ GallinaReify.Reify n @ GallinaReify.Reify m @ GallinaReify.Reify m' @ GallinaReify.Reify divstep_precompmod)
+         tt
+         (Some bounds).
+
+  Definition sdivstep_precomp (prefix : string)
+    : string * (Pipeline.ErrorT (Pipeline.ExtendedSynthesisResult _))
+    := Eval cbv beta in
+        FromPipelineToString
+          machine_wordsize prefix "divstep_precomp" divstep_precomp
+          (docstring_with_summary_from_lemma!
+             prefix
+             (fun fname => [text_before_function_name ++ fname ++ " returns the precomputed value for Bernstein-Yang-inversion (in montgomery form)."]%string)
+             (divstep_precomp_correct machine_wordsize n m valid from_montgomery_res)).
+
+  Definition divstep
+    := Pipeline.BoundsPipeline
+         false (* subst01 *)
+         None (* fancy *)
+         possible_values
+         (reified_divstep_gen
+            @ GallinaReify.Reify machine_wordsize @ GallinaReify.Reify sat_limbs @ GallinaReify.Reify n @ GallinaReify.Reify m)
+         (divstep_input)
+         (divstep_output).
+
+  Definition sdivstep (prefix : string)
+    : string * (Pipeline.ErrorT (Pipeline.ExtendedSynthesisResult _))
+    := Eval cbv beta in
+        FromPipelineToString
+          machine_wordsize prefix "divstep" divstep
+          (docstring_with_summary_from_lemma!
+             prefix
+             (fun fname : string => [text_before_function_name ++ fname ++ " computes a divstep."]%string)
+             (divstep_correct machine_wordsize n m valid from_montgomery_res)).
+
+  Lemma bounded_by_of_valid x
+        (H : valid x)
+    : ZRange.type.base.option.is_bounded_by (t:=base.type.list base.type.Z) (Some bounds) x = true.
+  Proof using curve_good.
+    pose proof use_curve_good as use_curve_good.
+    clear -H use_curve_good curve_good.
+    destruct H as [H _]; destruct_head'_and.
+    cbv [small] in H.
+    cbv [ZRange.type.base.option.is_bounded_by bounds saturated_bounds].
+    replace n with (List.length x) by now rewrite H, Partition.length_partition.
+    rewrite <- map_const, fold_andb_map_map1, fold_andb_map_iff.
+    cbv [ZRange.type.base.is_bounded_by is_bounded_by_bool lower upper type_base].
+    split; [ reflexivity | ].
+    intros *; rewrite combine_same, in_map_iff, Bool.andb_true_iff, !Z.leb_le.
+    intros; destruct_head'_ex; destruct_head'_and; subst *; cbn [fst snd].
+    match goal with
+    | [ H : In ?v x |- _ ] => revert v H
+    end.
+    rewrite H.
+    generalize (eval (n:=n) machine_wordsize x).
+    cbn [base.interp base.base_interp].
+    generalize n.
+    intro n'.
+    induction n' as [|n' IHn'].
+    { cbv [Partition.partition seq map In]; tauto. }
+    { intros *; rewrite Partition.partition_step, in_app_iff; cbn [List.In].
+      intros; destruct_head'_or; subst *; eauto; try tauto; [].
+      rewrite uweight_S by lia.
+      assert (0 < uweight machine_wordsize n') by now apply uwprops.
+      assert (0 < 2 ^ machine_wordsize) by auto with zarith.
+      assert (0 < 2 ^ machine_wordsize * uweight machine_wordsize n') by nia.
+      rewrite <- Z.mod_pull_div by lia.
+      rewrite Z.le_sub_1_iff.
+      auto with zarith. }
+  Qed.
+
+  (* XXX FIXME *)
+  Lemma bounded_by_prime_bounds_of_valid_gen lgr n' x
+        (Hlgr : 0 < lgr)
+        (Hs : s = 2^Z.log2 s)
+        (Hs' : s <= uweight lgr n')
+        (H : WordByWordMontgomery.valid lgr n' m x)
+    : ZRange.type.base.option.is_bounded_by (t:=base.type.list base.type.Z) (Some (List.map (fun v => Some r[0~>v]%zrange) (Partition.partition (uweight lgr) n' (s-1)))) x = true.
+  Proof using curve_good.
+    pose proof use_curve_good as use_curve_good.
+    clear -H use_curve_good curve_good Hlgr Hs Hs'.
+    destruct H as [H ?]; destruct_head'_and.
+    cbv [small] in H.
+    cbv [ZRange.type.base.option.is_bounded_by].
+    replace n' with (List.length x) by now rewrite H, Partition.length_partition.
+    rewrite fold_andb_map_map1, fold_andb_map_iff.
+    split; [ now autorewrite with distr_length | ].
+    cbv [ZRange.type.base.is_bounded_by is_bounded_by_bool lower upper].
+    rewrite H; autorewrite with distr_length.
+    intros [v1 v0]; cbn [fst snd].
+    rename x into x'.
+    generalize dependent (eval (n:=n') lgr x').
+    replace m with (s - c) in * by easy.
+    intro x; intros ??? H; subst x'.
+    eapply In_nth_error in H; destruct H as [i H].
+    rewrite nth_error_combine in H.
+    break_match_hyps; try discriminate; []; Option.inversion_option; Prod.inversion_prod; subst.
+    cbv [Partition.partition] in *.
+    apply nth_error_map_ex in Heqo; apply nth_error_map_ex in Heqo0; destruct Heqo as (?&?&?), Heqo0 as (?&?&?).
+    rewrite nth_error_seq in *.
+    break_match_hyps; try discriminate; Option.inversion_option; Prod.inversion_prod; subst.
+    rewrite ?Nat.add_0_l.
+    assert (0 <= x < s) by lia.
+    replace s with (2^Z.log2 s) by easy.
+    assert (1 < s) by lia.
+    assert (0 < Z.log2 s) by now apply Z.log2_pos.
+    assert (1 < 2^Z.log2 s) by auto with zarith.
+    generalize dependent (Z.log2 s); intro lgs; intros.
+
+    edestruct (uwprops lgr); try lia.
+    assert (forall i : nat, 0 <= uweight lgr i) by (intro z; specialize (weight_positive z); lia).
+    apply Bool.andb_true_intro; split; apply OrdersEx.Z_as_OT.leb_le;
+      [apply Z.div_nonneg | apply Z.div_le_mono_nonneg]; trivial.
+    apply Z.mod_pos_bound; trivial.
+
+    cbv [uweight].
+    cbv [weight].
+    rewrite Z.div_1_r.
+    rewrite Z.opp_involutive.
+    rewrite <-2Z.land_ones by nia.
+    rewrite Z.sub_1_r, <-Z.ones_equiv.
+    rewrite Z.land_ones_ones.
+    destruct ((lgs <? 0) || (lgr * Z.of_nat (S i) <? 0)) eqn:?.
+    { rewrite Z.land_ones, Z.ones_equiv, <-Z.sub_1_r by nia.
+      pose proof Z.le_max_r lgs (lgr*Z.of_nat (S i)).
+      etransitivity.
+      2:rewrite <- Z.sub_le_mono_r.
+      2:eapply Z.pow_le_mono_r; try lia; eassumption.
+      eapply Z.le_sub_1_iff, Z.mod_pos_bound, Z.pow_pos_nonneg; nia. }
+    rewrite (Z.ones_equiv (Z.min _ _)), <-Z.sub_1_r.
+    enough (Z.land x (Z.ones (lgr * Z.of_nat (S i))) < 2 ^ Z.min lgs (lgr * Z.of_nat (S i))) by lia.
+    eapply Testbit.Z.testbit_false_bound. nia.
+    intros j ?; assert (Z.min lgs (lgr * Z.of_nat (S i)) <= j) by lia.
+    rewrite Hs in *. revert H; intros.
+    rewrite <-(Z.mod_small x (2^lgs)) by lia.
+    rewrite OrdersEx.Z_as_OT.land_spec.
+    destruct (Zmin_irreducible lgs (lgr * Z.of_nat (S i))) as [HH|HH]; rewrite HH in *; clear HH.
+    { rewrite Z.mod_pow2_bits_high; trivial; lia. }
+    { rewrite OrdersEx.Z_as_DT.ones_spec_high, Bool.andb_false_r; trivial; nia. }
+  Qed.
+
+  Lemma length_of_valid lgr n' x
+        (H : WordByWordMontgomery.valid lgr n' m x)
+    : List.length x = n'.
+  Proof using Type.
+    destruct H as [H _]; rewrite H.
+    now autorewrite with distr_length.
+  Qed.
+
+  Lemma bounded_by_prime_bounds_of_valid x
+        (H : valid x)
+    : ZRange.type.base.option.is_bounded_by (t:=base.type.list base.type.Z) (Some prime_bounds) x = true.
+  Proof using curve_good.
+    pose proof use_curve_good as use_curve_good.
+    destruct_head'_and.
+    now apply bounded_by_prime_bounds_of_valid_gen.
+  Qed.
+
+  Lemma bounded_by_prime_bytes_bounds_of_bytes_valid x
+        (H : bytes_valid x)
+    : ZRange.type.base.option.is_bounded_by (t:=base.type.list base.type.Z) (Some prime_bytes_bounds) x = true.
+  Proof using curve_good.
+    pose proof use_curve_good as use_curve_good.
+    destruct_head'_and.
+    now apply bounded_by_prime_bounds_of_valid_gen.
+  Qed.
+
+  Lemma weight_bounded_of_bytes_valid x
+        (H : bytes_valid x)
+    : 0 <= eval 8 (n:=n_bytes) x < weight machine_wordsize 1 n.
+  Proof using curve_good.
+    cbv [bytes_valid] in H.
+    destruct H as [_ H].
+    pose proof use_curve_good.
+    cbv [uweight] in *; destruct_head'_and; lia.
+  Qed.
+
+  Local Ltac solve_extra_bounds_side_conditions :=
+    solve [ cbn [lower upper fst snd] in *; Bool.split_andb; Z.ltb_to_lt; lia
+          | cbv [valid small eval uweight n_bytes] in *; destruct_head'_and; auto
+          | now apply weight_bounded_of_bytes_valid
+          | eapply length_of_valid; eassumption ].
+
+  Hint Rewrite
+       (@eval_mulmod machine_wordsize n m r' m')
+       (@eval_squaremod machine_wordsize n m r' m')
+       (@eval_addmod machine_wordsize n m r' m')
+       (@eval_submod machine_wordsize n m r' m')
+       (@eval_oppmod machine_wordsize n m r' m')
+       (@eval_from_montgomerymod machine_wordsize n m r' m')
+       (@eval_to_montgomerymod machine_wordsize n m r' m')
+       (@eval_encodemod machine_wordsize n m r' m')
+       eval_to_bytesmod
+       eval_from_bytesmod
+       using solve [ eauto using length_of_valid | congruence | solve_extra_bounds_side_conditions ] : push_eval.
+  (* needed for making [autorewrite] fast enough *)
+  Local Opaque
+        WordByWordMontgomery.WordByWordMontgomery.onemod
+        WordByWordMontgomery.WordByWordMontgomery.from_montgomerymod
+        WordByWordMontgomery.WordByWordMontgomery.to_montgomerymod
+        WordByWordMontgomery.WordByWordMontgomery.mulmod
+        WordByWordMontgomery.WordByWordMontgomery.squaremod
+        WordByWordMontgomery.WordByWordMontgomery.encodemod
+        WordByWordMontgomery.WordByWordMontgomery.addmod
+        WordByWordMontgomery.WordByWordMontgomery.submod
+        WordByWordMontgomery.WordByWordMontgomery.oppmod
+        WordByWordMontgomery.WordByWordMontgomery.to_bytesmod.
+  Hint Unfold eval zeromod onemod : push_eval.
+
+  Local Ltac prove_correctness op_correct :=
+    let dont_clear H := first [ constr_eq H curve_good ] in
+    let Hres := match goal with H : _ = Success _ |- _ => H end in
+    let H := fresh in
+    pose proof use_curve_good as H;
+    (* I want to just use [clear -H Hres], but then I can't use any lemmas in the section because of COQBUG(https://github.com/coq/coq/issues/8153) *)
+    repeat match goal with
+           | [ H' : _ |- _ ]
+             => tryif first [ has_body H' | constr_eq H' H | constr_eq H' Hres | dont_clear H' ]
+             then fail
+             else clear H'
+           end;
+    cbv zeta in *;
+    destruct_head'_and;
+    let f := match type of Hres with ?f = _ => head f end in
+    try cbv [f] in *;
+    hnf;
+    PipelineTactics.do_unfolding;
+    try (let m := match goal with m := _ - Associational.eval _ |- _ => m end in
+         cbv [m] in * );
+    intros;
+    lazymatch goal with
+    | [ |- _ <-> _ ] => idtac
+    | [ |- _ = _ ] => idtac
+    | _ => split; [ | try split ];
+           cbv [small]
+    end;
+    PipelineTactics.use_compilers_correctness Hres;
+    repeat first [ reflexivity
+                 | now apply bounded_by_of_valid
+                 | now apply bounded_by_prime_bounds_of_valid
+                 | now apply bounded_by_prime_bytes_bounds_of_bytes_valid
+                 | now apply weight_bounded_of_bytes_valid
+                 | solve [ eapply op_correct; try eassumption; solve_extra_bounds_side_conditions ]
+                 | progress autorewrite with interp_gen_cache interp_extra
+                 | progress autorewrite with push_eval
+                 | progress autounfold with push_eval
+                 | progress autorewrite with distr_length in *
+                 | solve [ cbv [valid small eval uweight n_bytes] in *; destruct_head'_and; auto ] ].
+
+  (** TODO: DESIGN DECISION:
+
+        The correctness lemmas for most of the montgomery things are
+        parameterized over a `from_montgomery`.  When filling this in
+        for, e.g., mul-correctness, should I use `from_montgomery`
+        from arithmetic, or should I use `Interp
+        reified_from_montgomery` (the post-pipeline version), and take
+        in success of the pipeline on `from_montgomery` as well? *)
+
+  Lemma mul_correct res
+        (Hres : mul = Success res)
+    : mul_correct machine_wordsize n m valid from_montgomery_res (Interp res).
+  Proof using curve_good. prove_correctness mulmod_correct. Qed.
+
+  Lemma Wf_mul res (Hres : mul = Success res) : Wf res.
+  Proof using Type. prove_pipeline_wf (). Qed.
+
+  Lemma square_correct res
+        (Hres : square = Success res)
+    : square_correct machine_wordsize n m valid from_montgomery_res (Interp res).
+  Proof using curve_good. prove_correctness squaremod_correct. Qed.
+
+  Lemma Wf_square res (Hres : square = Success res) : Wf res.
+  Proof using Type. prove_pipeline_wf (). Qed.
+
+  Lemma add_correct res
+        (Hres : add = Success res)
+    : add_correct machine_wordsize n m valid from_montgomery_res (Interp res).
+  Proof using curve_good. prove_correctness addmod_correct. Qed.
+
+  Lemma Wf_add res (Hres : add = Success res) : Wf res.
+  Proof using Type. prove_pipeline_wf (). Qed.
+
+  Lemma sub_correct res
+        (Hres : sub = Success res)
+    : sub_correct machine_wordsize n m valid from_montgomery_res (Interp res).
+  Proof using curve_good. prove_correctness submod_correct. Qed.
+
+  Lemma Wf_sub res (Hres : sub = Success res) : Wf res.
+  Proof using Type. prove_pipeline_wf (). Qed.
+
+  Lemma opp_correct res
+        (Hres : opp = Success res)
+    : opp_correct machine_wordsize n m valid from_montgomery_res (Interp res).
+  Proof using curve_good. prove_correctness oppmod_correct. Qed.
+
+  Lemma Wf_opp res (Hres : opp = Success res) : Wf res.
+  Proof using Type. prove_pipeline_wf (). Qed.
+
+  Lemma from_montgomery_correct res
+        (Hres : from_montgomery = Success res)
+    : from_montgomery_correct machine_wordsize n m r' valid (Interp res).
+  Proof using curve_good. prove_correctness from_montgomerymod_correct. Qed.
+
+  Lemma Wf_from_montgomery res (Hres : from_montgomery = Success res) : Wf res.
+  Proof using Type. prove_pipeline_wf (). Qed.
+
+  Lemma to_montgomery_correct res
+        (Hres : to_montgomery = Success res)
+    : to_montgomery_correct machine_wordsize n m valid from_montgomery_res (Interp res).
+  Proof using curve_good. prove_correctness to_montgomerymod_correct. Qed.
+
+  Lemma Wf_to_montgomery res (Hres : to_montgomery = Success res) : Wf res.
+  Proof using Type. prove_pipeline_wf (). Qed.
+
+  Lemma nonzero_correct res
+        (Hres : nonzero = Success res)
+    : nonzero_correct machine_wordsize n m valid from_montgomery_res (Interp res).
+  Proof using curve_good. prove_correctness nonzeromod_correct. Qed.
+
+  Lemma Wf_nonzero res (Hres : nonzero = Success res) : Wf res.
+  Proof using Type. prove_pipeline_wf (). Qed.
+
+  Lemma to_bytes_correct res
+        (Hres : to_bytes = Success res)
+    : to_bytes_correct machine_wordsize n n_bytes m valid (Interp res).
+  Proof using curve_good. prove_correctness to_bytesmod_correct. Qed.
+
+  Lemma Wf_to_bytes res (Hres : to_bytes = Success res) : Wf res.
+  Proof using Type. prove_pipeline_wf (). Qed.
+
+  Lemma from_bytes_correct res
+        (Hres : from_bytes = Success res)
+    : from_bytes_correct machine_wordsize n n_bytes m valid bytes_valid (Interp res).
+  Proof using curve_good. prove_correctness eval_from_bytesmod_and_partitions. Qed.
+
+  Lemma Wf_from_bytes res (Hres : from_bytes = Success res) : Wf res.
+  Proof using Type. prove_pipeline_wf (). Qed.
+
+  Strategy -1000 [encode]. (* if we don't tell the kernel to unfold this early, then [Qed] seems to run off into the weeds *)
+  Lemma encode_correct res
+        (Hres : encode = Success res)
+    : encode_correct machine_wordsize n m valid from_montgomery_res (Interp res).
+  Proof using curve_good. prove_correctness encodemod_correct. Qed.
+
+  Lemma Wf_encode res (Hres : encode = Success res) : Wf res.
+  Proof using Type. prove_pipeline_wf (). Qed.
+
+  Strategy -1000 [zero]. (* if we don't tell the kernel to unfold this early, then [Qed] seems to run off into the weeds *)
+  Lemma zero_correct res
+        (Hres : zero = Success res)
+    : zero_correct machine_wordsize n m valid from_montgomery_res (Interp res).
+  Proof using curve_good. prove_correctness encodemod_correct. Qed.
+
+  Lemma Wf_zero res (Hres : zero = Success res) : Wf res.
+  Proof using Type. prove_pipeline_wf (). Qed.
+
+  Strategy -1000 [one]. (* if we don't tell the kernel to unfold this early, then [Qed] seems to run off into the weeds *)
+  Lemma one_correct res
+        (Hres : one = Success res)
+    : one_correct machine_wordsize n m valid from_montgomery_res (Interp res).
+  Proof using curve_good. prove_correctness encodemod_correct. Qed.
+
+  Lemma Wf_one res (Hres : one = Success res) : Wf res.
+  Proof using Type. prove_pipeline_wf (). Qed.
+
+  Local Opaque Pipeline.BoundsPipeline. (* need this or else [eapply Pipeline.BoundsPipeline_correct in Hres] takes forever *)
+  Lemma selectznz_correct res
+        (Hres : selectznz = Success res)
+    : selectznz_correct machine_wordsize n saturated_bounds (Interp res).
+  Proof using curve_good. Primitives.prove_correctness use_curve_good. Qed.
+
+  Lemma Wf_selectznz res (Hres : selectznz = Success res) : Wf res.
+  Proof using Type. prove_pipeline_wf (). Qed.
+
+  Section ring.
+    Context from_montgomery_res (Hfrom_montgomery : from_montgomery = Success from_montgomery_res)
+            mul_res    (Hmul    : mul    = Success mul_res)
+            add_res    (Hadd    : add    = Success add_res)
+            sub_res    (Hsub    : sub    = Success sub_res)
+            opp_res    (Hopp    : opp    = Success opp_res)
+            encode_res (Hencode : encode = Success encode_res)
+            zero_res   (Hzero   : zero   = Success zero_res)
+            one_res    (Hone    : one    = Success one_res).
+
+    Definition GoodT : Prop
+      := GoodT
+           machine_wordsize n m valid
+           (Interp from_montgomery_res)
+           (Interp mul_res)
+           (Interp add_res)
+           (Interp sub_res)
+           (Interp opp_res)
+           (Interp encode_res)
+           (Interp zero_res)
+           (Interp one_res).
+
+    Theorem Good : GoodT.
+    Proof using curve_good Hfrom_montgomery Hmul Hadd Hsub Hopp Hencode Hzero Hone.
+      pose proof use_curve_good; cbv zeta in *; destruct_head'_and.
+      eapply Good.
+      all: repeat first [ assumption
+                        | apply from_montgomery_correct
+                        | lia ].
+      all: hnf; intros.
+      all: push_Zmod; erewrite !(fun v Hv => proj1 (from_montgomery_correct _ Hfrom_montgomery v Hv)), <- !eval_from_montgomerymod; try eassumption; pull_Zmod.
+      all: repeat first [ assumption
+                        | lazymatch goal with
+                          | [ |- context[mul_res] ] => apply mul_correct
+                          | [ |- context[add_res] ] => apply add_correct
+                          | [ |- context[sub_res] ] => apply sub_correct
+                          | [ |- context[opp_res] ] => apply opp_correct
+                          | [ |- context[encode_res] ] => apply encode_correct
+                          | [ |- context[zero_res] ] => apply zero_correct
+                          | [ |- context[one_res] ] => apply one_correct
+                          end ].
+    Qed.
+  End ring.
+
+  Section for_stringification.
+    Local Open Scope string_scope.
+    Local Open Scope list_scope.
+
+    Definition known_functions
+      := [("mul", wrap_s smul);
+            ("square", wrap_s ssquare);
+            ("add", wrap_s sadd);
+            ("sub", wrap_s ssub);
+            ("opp", wrap_s sopp);
+            ("from_montgomery", wrap_s sfrom_montgomery);
+            ("to_montgomery", wrap_s sto_montgomery);
+            ("nonzero", wrap_s snonzero);
+            ("selectznz", wrap_s sselectznz);
+            ("to_bytes", wrap_s sto_bytes);
+            ("from_bytes", wrap_s sfrom_bytes);
+            ("one", wrap_s sone);
+            ("msat", wrap_s smsat);
+            ("divstep_precomp", wrap_s sdivstep_precomp);
+            ("divstep", wrap_s sdivstep)].
+
+    Definition valid_names : string := Eval compute in String.concat ", " (List.map (@fst _ _) known_functions).
+
+    (** Note: If you change the name or type signature of this
+          function, you will need to update the code in CLI.v *)
+    Definition Synthesize (comment_header : list string) (function_name_prefix : string) (requests : list string)
+      : list (synthesis_output_kind * string * Pipeline.ErrorT (list string))
+      := Primitives.Synthesize
+           machine_wordsize valid_names known_functions (fun _ => nil)
+           check_args
+           (ToString.comment_file_header_block
+              (comment_header
+                 ++ [""
+                     ; "Computed values:"]
+                 ++ (List.map
+                       (fun s => "  " ++ s)%string
+                       ((ToString.prefix_and_indent "eval z = " [seval "z"])
+                          ++ (ToString.prefix_and_indent "bytes_eval z = " [sbytes_eval "z"])
+                          ++ (ToString.prefix_and_indent "twos_complement_eval z = " [seval_twos_complement "z"])))))
+           function_name_prefix requests.
+  End for_stringification.
+End __.
+
+Module Export Hints.
+  Hint Opaque
+       mul
+       square
+       add
+       sub
+       opp
+       from_montgomery
+       to_montgomery
+       nonzero
+       to_bytes
+       from_bytes
+       encode
+       zero
+       one
+       selectznz
+  : wf_op_cache.
+  Hint Immediate
+       Wf_mul
+       Wf_square
+       Wf_add
+       Wf_sub
+       Wf_opp
+       Wf_from_montgomery
+       Wf_to_montgomery
+       Wf_nonzero
+       Wf_to_bytes
+       Wf_from_bytes
+       Wf_encode
+       Wf_zero
+       Wf_one
+       Wf_selectznz
+  : wf_op_cache.
+End Hints.
