src/PushButtonSynthesis/WordByWordMontgomeryGenericReificationCache.v
@@ -1,0 +1,286 @@
+(** * Push-Button Synthesis of Word-By-Word Montgomery: Reification Cache *)
+Require Import Coq.ZArith.ZArith.
+Require Import Coq.derive.Derive.
+Require Import Crypto.Util.Tactics.Head.
+Require Import Crypto.Arithmetic.Core.
+Require Import Crypto.Arithmetic.Freeze.
+Require Import Crypto.Arithmetic.ModOps.
+Require Import Crypto.Arithmetic.WordByWordMontgomery.
+Require Import Rewriter.Language.Language.
+Require Import Crypto.Language.API.
+Require Import Crypto.PushButtonSynthesis.ReificationCache.
+Local Open Scope Z_scope.
+
+Import
+  Language.Wf.Compilers
+  Language.Compilers
+  Language.API.Compilers.
+Import Compilers.API.
+
+Import Associational Positional.
+
+Local Set Keyed Unification. (* needed for making [autorewrite] fast, c.f. COQBUG(https://github.com/coq/coq/issues/9283) *)
+
+Module Export WordByWordMontgomery.
+  Import WordByWordMontgomery.WordByWordMontgomery.
+
+  Definition zeromod bitwidth n m m' := encodemod bitwidth n m m' 0.
+  Definition onemod bitwidth n m m' := encodemod bitwidth n m m' 1.
+  Definition evalmod bitwidth n := @eval bitwidth n.
+  Definition bytes_evalmod s := @eval 8 (bytes_n s).
+
+  (* we would do something faster, but it generally breaks extraction COQBUG(https://github.com/coq/coq/issues/7954) *)
+  Local Ltac precache_reify_faster _ :=
+    split;
+    [ let marker := fresh "marker" in
+      pose I as marker;
+      intros;
+      let LHS := lazymatch goal with |- ?LHS = _ => LHS end in
+      let reified_op_gen := lazymatch LHS with context[expr.Interp _ ?reified_op_gen] => reified_op_gen end in
+      subst reified_op_gen;
+      etransitivity;
+      [
+      | let opmod := match goal with |- _ = ?RHS => head RHS end in
+        cbv [opmod]; solve [ eauto with reify_cache_gen nocore ] ];
+      repeat lazymatch goal with
+             | [ H : _ |- _ ] => tryif constr_eq H marker then fail else revert H
+             end;
+      clear marker
+    | ].
+  Local Ltac cache_reify_faster_2arg _ :=
+    precache_reify_faster ();
+    [ lazymatch goal with
+      | [ |- forall bw n m m' v, ?interp ?ev bw n m m' v = ?interp' ?reified_mul_gen bw n m m' (@?A bw n m m' v) (@?B bw n m m' v) ]
+        => let rv := constr:(fun F bw n m m' v => (F bw n m m' (A bw n m m' v) (B bw n m m' v)):list Z) in
+           intros;
+           instantiate (1:=ltac:(let r := Reify rv in
+                                 refine (r @ reified_mul_gen)%Expr))
+      end;
+      reflexivity
+    | prove_Wf () ].
+  Local Ltac cache_reify_faster_1arg _ :=
+    precache_reify_faster ();
+    [ lazymatch goal with
+      | [ |- forall bw n m m', ?interp ?ev bw n m m' = ?interp' ?reified_op_gen bw n m m' (@?A bw n m m') ]
+        => let rv := constr:(fun F bw n m m' => (F bw n m m' (A bw n m m')):list Z) in
+           intros;
+           instantiate (1:=ltac:(let r := Reify rv in
+                                 refine (r @ reified_op_gen)%Expr))
+      end;
+      reflexivity
+    | prove_Wf () ].
+
+  (**
+<<
+#!/usr/bin/env python
+
+indent = '  '
+
+print((indent + '(' + r'''**
+<<
+%s
+>>
+*''' + ')\n') % open(__file__, 'r').read())
+
+for i in ('mul', 'add', 'sub', 'opp', 'to_bytes', 'from_bytes', 'nonzero', 'eval', 'bytes_eval'):
+    print((r'''%sDerive reified_%s_gen
+       SuchThat (is_reification_of reified_%s_gen %smod)
+       As reified_%s_gen_correct.
+Proof. Time cache_reify (). Time Qed.
+Global Hint Extern 1 (_ = _) => apply_cached_reification %smod (proj1 reified_%s_gen_correct) : reify_cache_gen.
+Hint Immediate (proj2 reified_%s_gen_correct) : wf_gen_cache.
+Hint Rewrite (proj1 reified_%s_gen_correct) : interp_gen_cache.
+Local Opaque reified_%s_gen. (* needed for making [autorewrite] not take a very long time *)''' % (indent, i, i, i, i, i, i, i, i, i)).replace('\n', '\n%s' % indent) + '\n')
+
+for i in ('square', 'encode', 'from_montgomery', 'to_montgomery'):
+    print((r'''%sDerive reified_%s_gen
+       SuchThat (is_reification_of reified_%s_gen %smod)
+       As reified_%s_gen_correct.
+Proof.
+  Time cache_reify ().
+  (* we would do something faster, but it breaks extraction COQBUG(https://github.com/coq/coq/issues/7954) *)
+  (* Time cache_reify_faster_2arg (). *)
+Time Qed.
+Global Hint Extern 1 (_ = _) => apply_cached_reification %smod (proj1 reified_%s_gen_correct) : reify_cache_gen.
+Hint Immediate (proj2 reified_%s_gen_correct) : wf_gen_cache.
+Hint Rewrite (proj1 reified_%s_gen_correct) : interp_gen_cache.
+Local Opaque reified_%s_gen. (* needed for making [autorewrite] not take a very long time *)''' % (indent, i, i, i, i, i, i, i, i, i)).replace('\n', '\n%s' % indent) + '\n')
+
+
+for i in ('zero', 'one'):
+    print((r'''%sDerive reified_%s_gen
+       SuchThat (is_reification_of reified_%s_gen %smod)
+       As reified_%s_gen_correct.
+Proof.
+  (* Time cache_reify (). *)
+  (* we do something faster *)
+  Time cache_reify_faster_1arg ().
+Time Qed.
+Global Hint Extern 1 (_ = _) => apply_cached_reification %smod (proj1 reified_%s_gen_correct) : reify_cache_gen.
+Hint Immediate (proj2 reified_%s_gen_correct) : wf_gen_cache.
+Hint Rewrite (proj1 reified_%s_gen_correct) : interp_gen_cache.
+Local Opaque reified_%s_gen. (* needed for making [autorewrite] not take a very long time *)''' % (indent, i, i, i, i, i, i, i, i, i)).replace('\n', '\n%s' % indent) + '\n')
+
+>>
+*)
+
+  Derive reified_mul_gen
+         SuchThat (is_reification_of reified_mul_gen mulmod)
+         As reified_mul_gen_correct.
+  Proof. Time cache_reify (). Time Qed.
+  Hint Extern 1 (_ = _) => apply_cached_reification mulmod (proj1 reified_mul_gen_correct) : reify_cache_gen.
+  Hint Immediate (proj2 reified_mul_gen_correct) : wf_gen_cache.
+  Hint Rewrite (proj1 reified_mul_gen_correct) : interp_gen_cache.
+  Local Opaque reified_mul_gen. (* needed for making [autorewrite] not take a very long time *)
+
+  Derive reified_add_gen
+         SuchThat (is_reification_of reified_add_gen addmod)
+         As reified_add_gen_correct.
+  Proof. Time cache_reify (). Time Qed.
+  Hint Extern 1 (_ = _) => apply_cached_reification addmod (proj1 reified_add_gen_correct) : reify_cache_gen.
+  Hint Immediate (proj2 reified_add_gen_correct) : wf_gen_cache.
+  Hint Rewrite (proj1 reified_add_gen_correct) : interp_gen_cache.
+  Local Opaque reified_add_gen. (* needed for making [autorewrite] not take a very long time *)
+
+  Derive reified_sub_gen
+         SuchThat (is_reification_of reified_sub_gen submod)
+         As reified_sub_gen_correct.
+  Proof. Time cache_reify (). Time Qed.
+  Hint Extern 1 (_ = _) => apply_cached_reification submod (proj1 reified_sub_gen_correct) : reify_cache_gen.
+  Hint Immediate (proj2 reified_sub_gen_correct) : wf_gen_cache.
+  Hint Rewrite (proj1 reified_sub_gen_correct) : interp_gen_cache.
+  Local Opaque reified_sub_gen. (* needed for making [autorewrite] not take a very long time *)
+
+  Derive reified_opp_gen
+         SuchThat (is_reification_of reified_opp_gen oppmod)
+         As reified_opp_gen_correct.
+  Proof. Time cache_reify (). Time Qed.
+  Hint Extern 1 (_ = _) => apply_cached_reification oppmod (proj1 reified_opp_gen_correct) : reify_cache_gen.
+  Hint Immediate (proj2 reified_opp_gen_correct) : wf_gen_cache.
+  Hint Rewrite (proj1 reified_opp_gen_correct) : interp_gen_cache.
+  Local Opaque reified_opp_gen. (* needed for making [autorewrite] not take a very long time *)
+
+  Derive reified_to_bytes_gen
+         SuchThat (is_reification_of reified_to_bytes_gen to_bytesmod)
+         As reified_to_bytes_gen_correct.
+  Proof. Time cache_reify (). Time Qed.
+  Hint Extern 1 (_ = _) => apply_cached_reification to_bytesmod (proj1 reified_to_bytes_gen_correct) : reify_cache_gen.
+  Hint Immediate (proj2 reified_to_bytes_gen_correct) : wf_gen_cache.
+  Hint Rewrite (proj1 reified_to_bytes_gen_correct) : interp_gen_cache.
+  Local Opaque reified_to_bytes_gen. (* needed for making [autorewrite] not take a very long time *)
+
+  Derive reified_from_bytes_gen
+         SuchThat (is_reification_of reified_from_bytes_gen from_bytesmod)
+         As reified_from_bytes_gen_correct.
+  Proof. Time cache_reify (). Time Qed.
+  Hint Extern 1 (_ = _) => apply_cached_reification from_bytesmod (proj1 reified_from_bytes_gen_correct) : reify_cache_gen.
+  Hint Immediate (proj2 reified_from_bytes_gen_correct) : wf_gen_cache.
+  Hint Rewrite (proj1 reified_from_bytes_gen_correct) : interp_gen_cache.
+  Local Opaque reified_from_bytes_gen. (* needed for making [autorewrite] not take a very long time *)
+
+  Derive reified_nonzero_gen
+         SuchThat (is_reification_of reified_nonzero_gen nonzeromod)
+         As reified_nonzero_gen_correct.
+  Proof. Time cache_reify (). Time Qed.
+  Hint Extern 1 (_ = _) => apply_cached_reification nonzeromod (proj1 reified_nonzero_gen_correct) : reify_cache_gen.
+  Hint Immediate (proj2 reified_nonzero_gen_correct) : wf_gen_cache.
+  Hint Rewrite (proj1 reified_nonzero_gen_correct) : interp_gen_cache.
+  Local Opaque reified_nonzero_gen. (* needed for making [autorewrite] not take a very long time *)
+
+  Derive reified_eval_gen
+         SuchThat (is_reification_of reified_eval_gen evalmod)
+         As reified_eval_gen_correct.
+  Proof. Time cache_reify (). Time Qed.
+  Hint Extern 1 (_ = _) => apply_cached_reification evalmod (proj1 reified_eval_gen_correct) : reify_cache_gen.
+  Hint Immediate (proj2 reified_eval_gen_correct) : wf_gen_cache.
+  Hint Rewrite (proj1 reified_eval_gen_correct) : interp_gen_cache.
+  Local Opaque reified_eval_gen. (* needed for making [autorewrite] not take a very long time *)
+
+  Derive reified_bytes_eval_gen
+         SuchThat (is_reification_of reified_bytes_eval_gen bytes_evalmod)
+         As reified_bytes_eval_gen_correct.
+  Proof. Time cache_reify (). Time Qed.
+  Hint Extern 1 (_ = _) => apply_cached_reification bytes_evalmod (proj1 reified_bytes_eval_gen_correct) : reify_cache_gen.
+  Hint Immediate (proj2 reified_bytes_eval_gen_correct) : wf_gen_cache.
+  Hint Rewrite (proj1 reified_bytes_eval_gen_correct) : interp_gen_cache.
+  Local Opaque reified_bytes_eval_gen. (* needed for making [autorewrite] not take a very long time *)
+
+  Derive reified_square_gen
+         SuchThat (is_reification_of reified_square_gen squaremod)
+         As reified_square_gen_correct.
+  Proof.
+    Time cache_reify ().
+    (* we would do something faster, but it breaks extraction COQBUG(https://github.com/coq/coq/issues/7954) *)
+    (* Time cache_reify_faster_2arg (). *)
+  Time Qed.
+  Hint Extern 1 (_ = _) => apply_cached_reification squaremod (proj1 reified_square_gen_correct) : reify_cache_gen.
+  Hint Immediate (proj2 reified_square_gen_correct) : wf_gen_cache.
+  Hint Rewrite (proj1 reified_square_gen_correct) : interp_gen_cache.
+  Local Opaque reified_square_gen. (* needed for making [autorewrite] not take a very long time *)
+
+  Derive reified_encode_gen
+         SuchThat (is_reification_of reified_encode_gen encodemod)
+         As reified_encode_gen_correct.
+  Proof.
+    Time cache_reify ().
+    (* we would do something faster, but it breaks extraction COQBUG(https://github.com/coq/coq/issues/7954) *)
+    (* Time cache_reify_faster_2arg (). *)
+  Time Qed.
+  Hint Extern 1 (_ = _) => apply_cached_reification encodemod (proj1 reified_encode_gen_correct) : reify_cache_gen.
+  Hint Immediate (proj2 reified_encode_gen_correct) : wf_gen_cache.
+  Hint Rewrite (proj1 reified_encode_gen_correct) : interp_gen_cache.
+  Local Opaque reified_encode_gen. (* needed for making [autorewrite] not take a very long time *)
+
+  Derive reified_from_montgomery_gen
+         SuchThat (is_reification_of reified_from_montgomery_gen from_montgomerymod)
+         As reified_from_montgomery_gen_correct.
+  Proof.
+    Time cache_reify ().
+    (* we would do something faster, but it breaks extraction COQBUG(https://github.com/coq/coq/issues/7954) *)
+    (* Time cache_reify_faster_2arg (). *)
+  Time Qed.
+  Hint Extern 1 (_ = _) => apply_cached_reification from_montgomerymod (proj1 reified_from_montgomery_gen_correct) : reify_cache_gen.
+  Hint Immediate (proj2 reified_from_montgomery_gen_correct) : wf_gen_cache.
+  Hint Rewrite (proj1 reified_from_montgomery_gen_correct) : interp_gen_cache.
+  Local Opaque reified_from_montgomery_gen. (* needed for making [autorewrite] not take a very long time *)
+
+  Derive reified_to_montgomery_gen
+         SuchThat (is_reification_of reified_to_montgomery_gen to_montgomerymod)
+         As reified_to_montgomery_gen_correct.
+  Proof.
+    Time cache_reify ().
+    (* we would do something faster, but it breaks extraction COQBUG(https://github.com/coq/coq/issues/7954) *)
+    (* Time cache_reify_faster_2arg (). *)
+  Time Qed.
+  Hint Extern 1 (_ = _) => apply_cached_reification to_montgomerymod (proj1 reified_to_montgomery_gen_correct) : reify_cache_gen.
+  Hint Immediate (proj2 reified_to_montgomery_gen_correct) : wf_gen_cache.
+  Hint Rewrite (proj1 reified_to_montgomery_gen_correct) : interp_gen_cache.
+  Local Opaque reified_to_montgomery_gen. (* needed for making [autorewrite] not take a very long time *)
+
+  Derive reified_zero_gen
+         SuchThat (is_reification_of reified_zero_gen zeromod)
+         As reified_zero_gen_correct.
+  Proof.
+    (* Time cache_reify (). *)
+    (* we do something faster *)
+    Time cache_reify_faster_1arg ().
+  Time Qed.
+  Hint Extern 1 (_ = _) => apply_cached_reification zeromod (proj1 reified_zero_gen_correct) : reify_cache_gen.
+  Hint Immediate (proj2 reified_zero_gen_correct) : wf_gen_cache.
+  Hint Rewrite (proj1 reified_zero_gen_correct) : interp_gen_cache.
+  Local Opaque reified_zero_gen. (* needed for making [autorewrite] not take a very long time *)
+
+  Derive reified_one_gen
+         SuchThat (is_reification_of reified_one_gen onemod)
+         As reified_one_gen_correct.
+  Proof.
+    Time cache_reify ().
+    (* Note that the following speed up breaks compilation of binaries /benjamin *)
+    (* we do something faster *)
+    (* Time cache_reify_faster_1arg (). *)
+  Time Qed.
+  Hint Extern 1 (_ = _) => apply_cached_reification onemod (proj1 reified_one_gen_correct) : reify_cache_gen.
+  Hint Immediate (proj2 reified_one_gen_correct) : wf_gen_cache.
+  Hint Rewrite (proj1 reified_one_gen_correct) : interp_gen_cache.
+  Local Opaque reified_one_gen. (* needed for making [autorewrite] not take a very long time *)
+End WordByWordMontgomery.
